theories/Completeness/my_files/my_kripkeModel.v
@@ -1,0 +1,300 @@
+From FOL Require Import FullSyntax Theories Deduction.FullSequentFacts Deduction.FragmentSequentFacts.
+
+
+From Undecidability.Synthetic Require Import Definitions DecidabilityFacts EnumerabilityFacts ListEnumerabilityFacts ReducibilityFacts.
+From Undecidability Require Import Shared.ListAutomation Shared.Dec FOL.Deduction.FullND.
+Require Import List Vector Lia.
+Import ListAutomationNotations ListAutomationHints ListAutomationInstances ListAutomationFacts.
+From FOL.Completeness Require Export TarskiCompleteness.
+From FOL.Utils Require Import MPFacts.
+Require Import Coq.Program.Equality.
+
+Require Import Undecidability.FOL.Semantics.Tarski.FullCore.
+
+(* ** Universal Models *)
+Section VariableDomainKripke.
+  Context {Σ_funcs : funcs_signature}.
+  Context {Σ_preds : preds_signature}.
+  
+  Arguments eval {_ _ _} _ _ _.
+  Arguments i_atom {_ _ _} _ _.
+  Arguments i_func {_ _ _} _ _.
+
+  (*Variable domain : Type.*)
+  Class kframe :=
+      { 
+        domain : Type;
+        nodes : Type ;
+        world : nodes -> domain -> Prop;
+
+        reachable : nodes -> nodes -> Prop ;
+        reach_refl u : reachable u u ;
+        reach_tran u v w : reachable u v -> reachable v w -> reachable u w ;
+
+        monotone u v : reachable u v ->  forall x:domain, world u x ->  world v x ;
+      }.
+  Context {frm : kframe}.
+
+  Definition in_dom (u : nodes) (n : nat) (vv: (t _ n)): Prop :=
+    forall x, In x vv -> (world u) x.
+
+  Lemma in_dom_mon (u v: nodes)(n : nat) (vv: (t _ n)) :
+      reachable u v -> in_dom u vv -> in_dom v vv.
+  Proof.
+    unfold in_dom.
+    eauto using monotone.
+  Qed. 
+
+  Class kmodel := {
+        I : nodes -> interp domain;
+        
+        mon_f (u v:nodes) (f: syms) (vv: (t domain (ar_syms f))) (reach : reachable u v) (a : in_dom u vv): 
+           i_func (I u) f vv = i_func (I v) f vv;
+
+        k_f_wellDef u f vv (vv_in_dom : (in_dom u vv)): world u (i_func (I u) f vv) (*/\  in_dom u vv*);
+
+        mon_P (u v:nodes) (P: preds) (vv: (t domain (ar_preds P))) (reach : reachable u v) (a : in_dom u vv): 
+           i_atom (I u) P vv -> i_atom (I v) P vv;
+
+        k_P_wellDef u P vv: i_atom (I u) P vv -> in_dom u vv;
+      }.
+
+   Context {M : kmodel}.
+
+   Fixpoint ksat{ff : falsity_flag}(u: nodes)(rho : nat -> domain)(phi : form) : Prop :=
+      match phi with
+      | atom P vv => i_atom (I u) P (map (eval (I u) rho) vv) 
+      | falsity => False
+      | bin Impl phi psi => forall v, reachable u v -> ksat v rho phi -> ksat v rho psi
+      | bin Conj phi psi => (ksat u rho phi) /\ (ksat u rho psi)
+      | bin Disj phi psi => (ksat u rho phi) \/ (ksat u rho psi) 
+      | quant All phi => forall v, reachable u v -> forall j : domain, world v j -> ksat v (j .: rho) phi 
+      | quant Ex phi => exists j: domain, world u j  /\  ksat u (j .: rho) phi
+      end.
+
+Definition good (u : nodes) (rho : nat -> domain)  := 
+      (forall n : nat, world u (rho n)).
+
+Lemma good_eval (u : nodes) (rho : nat -> domain) (t : term):
+  good u rho -> world u (eval (I u) rho t). 
+  Proof.
+    intros. induction t.
+    * eauto.
+    * cbn.  
+      apply k_f_wellDef.  unfold in_dom.
+      intros x [a [b <-]] % vector_in_map. now apply IH.
+Qed.
+
+   Lemma good_mon (u v: nodes) (rho : nat -> domain) :
+      good u rho -> reachable u v -> good v rho.
+    Proof.
+      unfold good.
+      intros.
+      eauto using monotone.
+    Qed.
+
+ Lemma eval_mon_t (u v: nodes) (rho : nat -> domain)(t: term):
+      @good u rho -> reachable u v -> eval (I u) rho t = eval (I v) rho t.
+      intros. induction t. 
+      * simpl. reflexivity.
+      * simpl.
+        erewrite map_ext_in.
+        apply mon_f. apply H0. unfold in_dom.
+        intros x [a [b <-]] % vector_in_map. 
+        erewrite <- IH.  
+        now eapply good_eval.
+        apply b. apply IH.
+  Qed.     
+
+  Lemma eval_mon (u v: nodes) (rho : nat -> domain):
+      @good u rho -> reachable u v -> forall t: term, eval (I u) rho t = eval (I v) rho t.
+  Proof.
+    intros.
+    now apply eval_mon_t.
+  Qed.
+
+  Lemma map_eval_vv (u v: nodes) (rho : nat -> domain) (n : nat)(vv: t term n):
+      @good u rho -> reachable u v -> map (eval (I u) rho) vv = map (eval (I v) rho) vv.
+  Proof.
+    intros.
+    eapply map_ext. now eapply eval_mon.
+  Qed.
+
+  Lemma in_dom_mix (u v: nodes) (rho : nat -> domain) (n : nat)(vv: t term n):
+      @good u rho -> reachable u v -> in_dom u (map (eval (I u) rho) vv) -> in_dom u (map (eval (I v) rho) vv).
+  Proof.
+    intros. 
+    erewrite map_ext_in. 
+    erewrite <- map_eval_vv. apply H1.
+    apply H. apply H0.  
+    intros. 
+    eauto using eval_mon, good_mon, reach_refl. 
+  Qed.
+
+   Lemma good_shift (u: nodes)(rho : nat -> domain)(j : domain):
+      good u rho -> world u j -> good u (j .: rho).
+    Proof.
+      unfold good.
+      intros H wj n.
+      induction n; simpl; auto.
+    Qed.  
+
+    Lemma shift_ext (rho xi: nat -> domain)(j : domain): 
+      (forall x : nat, rho x = xi x) -> forall x: nat, (j .: rho) x = (j .: xi) x.
+    Proof.
+      intros. unfold scons. destruct x. reflexivity. apply H. 
+    Qed.
+    
+    Lemma good_ext (u: nodes) (rho xi: nat -> domain):
+      good u rho ->  (forall x, rho x = xi x) -> good u xi.
+    Proof.
+      intros. unfold good in *. intros. rewrite <- H0. apply H.
+    Qed.
+
+    Lemma good_comp (u: nodes)(rho: nat -> domain)(xi : nat -> term):
+     good u rho -> good u (xi >> eval (I u) rho).
+    Proof.
+    intros. unfold good. intros. eapply good_eval. apply H.
+    Qed.
+
+    Lemma good_comp_reach (u v: nodes)(rho: nat -> domain)(xi : nat -> term):
+      good u rho -> reachable u v -> good v (xi >> eval (I u) rho).
+    Proof.
+    unfold good. intros. eapply good_mon; now eauto using good_comp. 
+    Qed.
+
+      
+  
+End VariableDomainKripke.
+
+Arguments kmodel {_ _ _}.
+
+#[local] Ltac comp := repeat (progress (cbn in *; autounfold in *)).
+
+Section KripkeSat.
+  Context {Σf : funcs_signature} {Σp : preds_signature}.
+  Context {frm : kframe}.
+
+  Context {M : kmodel}.
+(* Context {ff : falsity_flag} *)
+
+
+
+    
+    Arguments eval {_ _ _} _ _ _.
+
+    Lemma ksat_mon {ff : falsity_flag}(u v: nodes) (rho : nat -> domain) (phi : form) : 
+      good u rho -> reachable u v -> ksat u rho phi -> ksat v rho phi.
+    Proof.
+      revert rho. 
+      induction phi; intros rho gd R H; cbn.
+      * apply H.
+      * unfold ksat in H.
+        apply (mon_P R). 
+          ++ erewrite map_eval_vv; try apply reach_refl; eauto using in_dom_mix, k_P_wellDef, good_mon. 
+          ++ erewrite <- map_eval_vv; eauto. 
+      * destruct b0.
+        + destruct H; split; eauto.
+        + destruct H; [left | right]; eauto. 
+        + simpl in H. intros w Rw IH. eauto using reach_tran. 
+      * destruct q; simpl in H.
+        + intros w Rw j wj. eauto using reach_tran. 
+        + destruct H as (j, H). exists j. split.
+          ++ eapply monotone; now eauto.
+          ++ eapply IHphi. now eapply good_shift. apply R. apply H.
+    Qed.
+
+    Lemma ksat_iff {ff : falsity_flag}(u v: nodes) (rho : nat -> domain) (phi : form):
+      good u rho -> (ksat u rho phi <-> forall v (H : reachable u v), ksat v rho phi).
+    Proof.
+      split; intros.
+      - eapply ksat_mon; eauto.
+      - auto using reach_refl.
+    Qed.
+    
+  Notation "rho  '⊩(' u ')'  phi" := (ksat _ u rho phi) (at level 20).
+  Notation "rho '⊩(' u , M ')' phi" := (@ksat _ _ _ M _ u rho phi) (at level 20).
+  
+Arguments ksat {_ _ _} _ _ _, _ _ _ _ _ _.
+  Hint Resolve reach_refl : core.
+
+  Section Substs.
+
+    Lemma ksat_ext {ff : falsity_flag}(u: nodes)(rho xi: nat -> domain)(phi: form):
+      good u rho -> (forall x, rho x = xi x) -> (rho ⊩(u,M) phi <-> xi ⊩(u,M) phi).
+    Proof.
+      induction phi as [ | b P v | | ] in rho, xi, u |-*; intros gdu Hext; comp.
+      - tauto.
+      - erewrite Vector.map_ext. reflexivity. intros t. now apply eval_ext.
+      - destruct b0;  split; intros H; try intros v Huv; rewrite IHphi1, IHphi2; eauto using good_ext, good_mon.  
+      - destruct q.
+        + split; intros; erewrite IHphi; eauto using good_mon, shift_ext, good_shift, good_ext.
+        + split; intros; repeat destruct H; exists x; split;
+          [ | eapply (IHphi _ (x .: rho) (x .: xi)) |  | eapply (IHphi _ (x .: xi) (x .: rho))]; 
+          try eauto using good_shift, good_ext; induction x0; eauto.
+    Qed.
+
+   Lemma eval_shift_up (u: nodes)(rho: nat -> domain)(xi : nat -> term)(j : domain)(n: nat):
+    ( j .: xi >> eval (I u) rho) n = ((up xi) >> eval (I u) (j .:rho)) n.
+   Proof.
+     intros; induction n; cbn.
+     * reflexivity.
+     * unfold ">>" in *. now erewrite <- eval_up. 
+   Qed.
+
+   Lemma eval_mon_shift_up (u v: nodes)(rho: nat -> domain)(xi : nat -> term)(j : domain)(n: nat):
+    good u rho -> reachable u v ->
+    ( j .: xi >> eval (I u) rho) n = ((up xi) >> eval (I v) (j .:rho)) n.
+   Proof.
+     intros; induction n; cbn.
+     * reflexivity.
+     * unfold ">>" in *. erewrite eval_mon; [now erewrite <- eval_up | | ]; auto.
+   Qed.
+    
+    Lemma ksat_comp {ff : falsity_flag}(u: nodes)(rho: nat -> domain)(xi : nat -> term)(phi: form) :
+      good u rho -> (rho ⊩(u,M) phi[xi] <-> (xi >> eval (I u) rho) ⊩(u,M) phi).
+    Proof.
+      induction phi as [ | b P v | | ] in rho, xi, u |-*; comp.
+      - tauto.
+      - erewrite Vector.map_map. erewrite Vector.map_ext. 2: apply eval_comp. reflexivity.
+      - destruct b0; intros.
+        + split; [split; [eapply IHphi1| eapply IHphi2] | split; [eapply IHphi1| eapply IHphi2]]; now eauto.
+        + split; intros; destruct H0; [left | right | left | right]; 
+          [eapply IHphi1| eapply IHphi2 | eapply IHphi1| eapply IHphi2]; now eauto. 
+        + split; intros.
+          ++ eapply ksat_ext; [now eapply good_comp_reach| intros | eapply IHphi2]; 
+            [ eapply eval_mon | | apply (H0 v H1);  eapply IHphi1].
+            5: eapply ksat_ext. 7: eapply H2. 6: intros; unfold ">>"; erewrite <- (eval_mon_t (xi x)). 
+            all: now eauto using good_mon, good_comp.
+          ++ eapply IHphi2; [ | eapply ksat_ext]; [| |intros | eapply H0].
+            5: eapply ksat_ext. 7: eapply IHphi1. 8: eapply H2. 5: intros. 6: intros.
+            all: unfold ">>" . 
+            3: erewrite <- (eval_mon_t (xi x)). 
+            all: eauto using good_comp_reach, eval_mon, good_comp, good_mon.
+      - destruct q; split; intros; try  destruct H0 as (j, (H0, H1)); try exists j; try split; try apply H0.
+          * eapply ksat_ext; try eapply IHphi; try eapply H0;
+            [unfold good; intros; eapply good_shift| intros |  |  | ]; 
+            eauto using good_comp_reach, good_shift, good_mon. now eapply eval_mon_shift_up. 
+          * eapply IHphi; [ | eapply ksat_ext]; [ | | intros | eapply H0]. 
+            3: erewrite eval_mon_shift_up.  all: eauto using good_shift, good_mon, good_comp, H2.
+          * eapply ksat_ext; [ |intros; now eapply eval_mon_shift_up |eapply IHphi]; 
+            eauto using good_shift, good_comp.
+          * eapply IHphi; [| eapply ksat_ext]; [ | |intros| eapply H1]; 
+            eauto using good_shift, good_comp, eval_shift_up.          
+    Qed.
+
+    Lemma ksat_shift {ff : falsity_flag}(u: nodes)(rho: nat -> domain)(phi: form):
+    good u rho-> forall j: domain, world u j -> (
+    rho ⊩( u, M) phi <-> (j.: rho)  ⊩( u, M) phi [↑]).
+    Proof.
+      split; intros.
+      rewrite ksat_comp; eauto using good_shift.
+      rewrite ksat_comp in H1. eapply ksat_ext. all: now eauto using good_shift.
+    Qed.
+
+  End Substs.
+
+End KripkeSat. 
+
+  Notation "rho  '⊩(' u ')'  phi" := (ksat _ u rho phi) (at level 20).
+  Notation "rho '⊩(' u , M ')' phi" := (@ksat _ _ _ M _ u rho phi) (at level 20).
